\chapter{Maths}

\section{Syntax}

%%%%%%%%%%%%%%%%%%%%%%%%%%%%%%%%%%%%%%%%%%%%%%%%
\begin{LaTeXsource}[Symbols]
\begin{verbatim}
$$ \int_1^2 X \mathrm{d} X = [ X^2 / 2]_1^2 = 3/2 $$
$$ n! \approx \sqrt{2 \pi n} (n / e)^n $$
\end{verbatim}
\end{LaTeXsource}

\begin{Results}
$$ \int_1^2 X \mathrm{d} X = [ X^2 / 2]_1^2 = 3/2 $$
$$ n! \approx \sqrt{2 \pi n} (n / e)^n $$
\end{Results}

\pagebreak
%%%%%%%%%%%%%%%%%%%%%%%%%%%%%%%%%%%%%%%%%%%%%%%%

\begin{LaTeXsource}[Boxing]
\begin{verbatim}
$$
\ln(n\,!) = n \ln(n) - n
    +   \frac{1}{2} \ln(2 \pi n)
    +   \sum_{k=1}^K
        \frac{  (-1)^{k+1} B_{k+1}  }{  k (k+1) n^{k}  }
    +   \mathcal{O}
        \left(  \frac{1}{n^{K+1}}  \right)
$$
$$
\lim_{n\to +\infty }{
n\,!
\over
{\sqrt{2\pi n}}\;
\left( \frac{n}{\rm e} \right)^n
}=1
$$
\end{verbatim}
\end{LaTeXsource}

\begin{Results}
$$
\ln(n\,!) =
        n \ln(n) - n
    +   \frac{1}{2} \ln(2 \pi n)
    +   \sum_{k=1}^K
        \frac{ (-1)^{k+1} B_{k+1} }{ k (k+1) n^{k} }
    +   \mathcal{O}
        \left(
            \frac{1}{n^{K+1}}
        \right)
$$
$$
\lim_{n\to +\infty }{
n\,!
\over
{\sqrt{2\pi n}}\;\left(\frac{n}{\rm e} \right)^n
}=1
$$
\end{Results}

\section{Display}

%%%%%%%%%%%%%%%%%%%%%%%%%%%%%%%%%%%%%%%%%%%%%%%%
\begin{LaTeXsource}[Inline]
\begin{verbatim}
Mathematical expression in the text
$\vec{\nabla} \cdot \vec{E} = \frac{\rho}{\varepsilon _{0}}$
is possible.
\end{verbatim}
\end{LaTeXsource}

\begin{Results}
Mathematical expression in the text
${\vec  {\nabla }}\cdot {\vec  {E}}={\frac  {\rho }{\varepsilon _{0}}}$
is possible.
\end{Results}

%%%%%%%%%%%%%%%%%%%%%%%%%%%%%%%%%%%%%%%%%%%%%%%%
\begin{LaTeXsource}[Displayed]
\begin{verbatim}
I can reference the equation \ref{myEquation}
that comes hereafter:

\begin{equation}\label{myEquation}
  \oint _C \vec{E} \cdot \mathrm{d} \vec{l}  =
- \iint _S \frac{\partial \vec{B}}{\partial{t}}
    \cdot \mathrm{d} \vec{S}
\end{equation}
\end{verbatim}
\end{LaTeXsource}

\begin{Results}
I can reference the equation \ref{myEquation} that comes hereafter.

\begin{equation}\label{myEquation}
\oint _C \vec{E} \cdot \mathrm{d} \vec{l}  =
- \iint _S \frac{\partial \vec{B}}{\partial{t}} \cdot \mathrm{d} \vec{S}
\end{equation}
\end{Results}
